again add some stronger assumptions to end-to-end lemma
the non-passive and passive global states must coincide on the constants, which means the constants have to be constrained at the beginning. This assumption was removed in an earlier commit but now has been added in a new way. Instead of forcing the variable relation to map every constant, we directly encode the assumption in the construction of the initial set.

BoogieLang/PassificationEndToEnd.thy
@@ -5,7 +5,7 @@ begin
 fun initial_set :: "'a absval_ty_fun \<Rightarrow> passive_rel \<Rightarrow> var_context \<Rightarrow> var_context \<Rightarrow> rtype_env \<Rightarrow> 'a nstate \<Rightarrow> ('a nstate) set"
   where "initial_set A R \<Lambda> \<Lambda>' \<Omega> ns = 
               {u. state_typ_wf A \<Omega> (local_state u) (snd \<Lambda>') \<and> state_typ_wf A \<Omega> (global_state u) (fst \<Lambda>') \<and>
-              (\<forall>x y. R x = Some (Inl y) \<longrightarrow> lookup_var \<Lambda> ns x = lookup_var \<Lambda>' u y) \<and>
+              (\<forall>x y. R x = Some (Inl y) \<longrightarrow> lookup_var \<Lambda> ns x = lookup_var \<Lambda>' u y) \<and> (\<forall> x y. map_of (fst \<Lambda>) x = Some y \<longrightarrow> (global_state u) x = (global_state ns) x) \<and>
               binder_state u = Map.empty}"
 
 fun initial_state_local :: "'a absval_ty_fun \<Rightarrow> rtype_env \<Rightarrow> passive_rel \<Rightarrow> var_context \<Rightarrow> var_context \<Rightarrow> 'a nstate \<Rightarrow> 'a named_state"
@@ -61,11 +61,16 @@ lemma init_state_elem_init_set:
           RelTy:"\<And>x y. R x = Some (Inl y) \<Longrightarrow> lookup_var_ty \<Lambda> x = lookup_var_ty \<Lambda>' y" and
           RelWt:"rel_well_typed A \<Lambda> \<Omega> R ns" and
           InjAssm:"inj_on_defined R" and
+          GlobalsSame: "fst \<Lambda> = fst \<Lambda>'" and
+          WellTyp: "(state_typ_wf A \<Omega> (global_state ns) (fst \<Lambda>))" and
+       (* since the initial state's global state is the same as for n_s (otherwise the axiom assumption cannot be satisfied)
+          the lemma requires that that the R maps globals to globals (otherwise it cannot be shown that ns and u respect R)*)
+          RelGlobalsSame: "\<forall>x y. R x = Some (Inl y) \<longrightarrow> map_of (fst \<Lambda>') y \<noteq> None \<longrightarrow> x = y" and 
        (* no shadowing *)
           ConstsDisj:"set (map fst (fst \<Lambda>')) \<inter> set (map fst (snd \<Lambda>)) = {}" and
           ConstsDisj2:"set (map fst (fst \<Lambda>')) \<inter> set (map fst (snd \<Lambda>')) = {}"
         shows "\<lparr>old_global_state = Map.empty, 
-               global_state = (initial_state_global A \<Omega> R \<Lambda> \<Lambda>' ns), 
+               global_state = global_state ns, 
                local_state = (initial_state_local A \<Omega> R \<Lambda> \<Lambda>' ns), 
                binder_state = Map.empty \<rparr> \<in> initial_set A R \<Lambda> \<Lambda>' \<Omega> ns" (is "?u \<in> ?U")
 proof (simp only: initial_set.simps, rule, intro conjI)
@@ -96,36 +101,7 @@ proof (simp only: initial_set.simps, rule, intro conjI)
     qed
   qed
 next
-  show "state_typ_wf A \<Omega> (global_state ?u) (fst \<Lambda>')"
-    unfolding state_typ_wf_def
-  proof ((rule allI)+, rule impI)
-    fix y \<tau>
-    assume global_y:"map_of (fst \<Lambda>') y = Some \<tau>"
-    from this moreover have "map_of (snd \<Lambda>') y = None" using ConstsDisj2
-      by (metis disjoint_iff_not_equal list.set_map map_of_eq_None_iff option.distinct(1)) 
-    ultimately have LookupTyY:"lookup_var_ty \<Lambda>' y = Some \<tau>"
-      by (simp add: lookup_var_ty_global) 
-    from \<open>map_of (fst \<Lambda>') y = Some \<tau>\<close> have "(y, \<tau>) \<in> set (fst \<Lambda>')" 
-      by (simp add: map_of_SomeD) 
-    show "map_option (type_of_val A) (global_state ?u y) = Some (instantiate \<Omega> \<tau>)"
-    proof (cases "\<exists>x. R x = Some (Inl y)")
-      case True
-      from this obtain x where "R x = Some (Inl y)" by auto
-      hence LookupUY:"global_state ?u y = lookup_var \<Lambda> ns x"
-        by (metis \<open>R x = Some (Inl y)\<close> initial_state_global_lookup[OF InjAssm] global_y nstate.select_convs(2))
-      from RelTy RelWt obtain v where
-              "lookup_var \<Lambda> ns x = Some v" and "type_of_val A v = instantiate \<Omega> \<tau>"
-        unfolding rel_well_typed_def using LookupTyY \<open>R x = Some (Inl y)\<close>
-        by fastforce 
-      thus ?thesis using LookupUY by auto
-    next
-      case False
-      hence "global_state ?u y = Some (val_of_type A (instantiate \<Omega> \<tau>))"
-        by (simp add: global_y) 
-      thus ?thesis using  False LookupTyY Closed val_of_type_correct NonEmptyTypes
-        by blast      
-    qed
-  qed
+  show "state_typ_wf A \<Omega> (global_state ?u) (fst \<Lambda>')" using WellTyp GlobalsSame by simp
 next
   show "\<forall> x y. R x = Some (Inl y) \<longrightarrow> lookup_var \<Lambda> ns x = lookup_var \<Lambda>' ?u y"
   proof (rule+)
@@ -142,10 +118,14 @@ next
         by (simp add: lookup_var_ty_global_3)
       from True have "lookup_var \<Lambda>' ?u y = global_state ?u y"
         by (simp add: lookup_var_def)
-      hence "\<dots> = (lookup_var \<Lambda> ns (SOME z. R z = Some (Inl y)))" using \<open>R x = Some (Inl y)\<close> True  global_y
-        by auto
-      then show ?thesis using InjAssm \<open>R x = Some (Inl y)\<close> 
-        by (metis \<open>lookup_var \<Lambda>' ?u y = global_state ?u y\<close> global_y initial_state_global_lookup nstate.select_convs(2))
+      hence lookup_global_u:"lookup_var \<Lambda>' ?u y = global_state ns y" by simp
+      from global_y have "map_of (fst \<Lambda>) y = Some \<tau>" using GlobalsSame by simp
+      moreover from this have "map_of (snd \<Lambda>) y = None" using ConstsDisj 
+        by (metis GlobalsSame disjoint_iff_not_equal list.set_map map_of_eq_None_iff option.distinct(1))
+      ultimately have "lookup_var \<Lambda> ns y = (global_state ns) y" by (simp add: lookup_var_def)
+      with lookup_global_u have "lookup_var \<Lambda> ns y = lookup_var \<Lambda>' ?u y" by simp
+      moreover from \<open>map_of (fst \<Lambda>') y = Some \<tau>\<close> \<open>R x = Some (Inl y)\<close> RelGlobalsSame have "x = y" by simp
+      ultimately show ?thesis by simp
     next
       case False
       hence "lookup_var \<Lambda>' ?u y = local_state ?u y"
@@ -155,6 +135,8 @@ next
         by (metis False \<open>lookup_var \<Lambda>' ?u y = local_state ?u y\<close> nstate.select_convs(3) option.collapse)
     qed
   qed
+next
+  show "\<forall>x y. map_of (fst \<Lambda>) x = Some y \<longrightarrow> (global_state ?u) x = (global_state ns) x" by simp
 next
   show "binder_state ?u = Map.empty"
     by simp
@@ -166,13 +148,16 @@ lemma init_set_non_empty:
           RelTy:"\<And>x y. R x = Some (Inl y) \<Longrightarrow> lookup_var_ty \<Lambda> x = lookup_var_ty \<Lambda>' y" and
           RelWt:"rel_well_typed A \<Lambda> \<Omega> R ns" and
           InjAssm:"inj_on_defined R" and
+          GlobalsSame: "fst \<Lambda> = fst \<Lambda>'" and
+          WellTyp: "(state_typ_wf A \<Omega> (global_state ns) (fst \<Lambda>))" and
+          RelGlobalsSame: "\<forall>x y. R x = Some (Inl y) \<longrightarrow> map_of (fst \<Lambda>') y \<noteq> None \<longrightarrow> x = y" and 
           ConstsDisj:"set (map fst (fst \<Lambda>')) \<inter> set (map fst (snd \<Lambda>)) = {}" and
           ConstsDisj2:"set (map fst (fst \<Lambda>')) \<inter> set (map fst (snd \<Lambda>')) = {}"
   shows "initial_set A R \<Lambda> \<Lambda>' \<Omega> ns \<noteq> {}"
   using assms init_state_elem_init_set by blast
 
-lemma init_state_dependent:"dependent A \<Lambda>' \<Omega> (initial_set A R \<Lambda> \<Lambda>' \<Omega> ns) (rel_range R)" 
-         (is "dependent A \<Lambda>' \<Omega> ?U (rel_range R)")
+lemma init_state_dependent:"dependent A \<Lambda>' \<Omega> (initial_set A R \<Lambda> \<Lambda>' \<Omega> ns) ((rel_range R) \<union> set (map fst (fst \<Lambda>)))" 
+         (is "dependent A \<Lambda>' \<Omega> ?U ((rel_range R) \<union> set (map fst (fst \<Lambda>))) ")
   unfolding dependent_def closed_set_ty_def
   proof (rule ballI, rule allI, rule allI, rule impI, rule conjI[OF _ impI[OF allI[OF impI]]])
     fix u \<tau> d
@@ -190,7 +175,7 @@ lemma init_state_dependent:"dependent A \<Lambda>' \<Omega> (initial_set A R \<L
           Rel1: "(\<forall>x y. R x = Some (Inl y) \<longrightarrow> lookup_var \<Lambda> ns x = lookup_var \<Lambda>' u y)" and
           Binder1: "binder_state u = Map.empty" by auto
     assume LookupTy:"lookup_var_ty \<Lambda>' d = Some \<tau>"
-    assume "d \<notin> rel_range R"
+    assume dNotElem:"d \<notin> rel_range R \<union> set (map fst (fst \<Lambda>))"
     assume TypV:"type_of_val A v = instantiate \<Omega> \<tau>"
     have S1Upd:"state_typ_wf A \<Omega> (local_state (update_var \<Lambda>' u d v)) (snd \<Lambda>')"
       unfolding state_typ_wf_def
@@ -246,25 +231,32 @@ lemma init_state_dependent:"dependent A \<Lambda>' \<Omega> (initial_set A R \<L
       assume "R x = Some (Inl y)"
       show "lookup_var \<Lambda> ns x = lookup_var \<Lambda>' (update_var \<Lambda>' u d v) y"
         apply (cases "d = y")
-        using \<open>R x = Some (Inl y)\<close> \<open>d \<notin> rel_range R\<close> 
+        using \<open>R x = Some (Inl y)\<close> dNotElem
          apply (simp add: rel_range_def)
         using Rel1 \<open>R x = Some (Inl y)\<close> 
         apply simp
         done
-    qed      
+    qed 
+    have GlobalConstraint: "\<forall>x y. map_of (fst \<Lambda>) x = Some y \<longrightarrow> global_state (update_var \<Lambda>' u d v) x = global_state ns x"
+    proof (rule+)
+      fix x y
+      assume "map_of (fst \<Lambda>) x = Some y"
+      hence "d \<noteq> x" using dNotElem
+        by (metis UnCI domI dom_map_of_2)
+      thus "global_state (update_var \<Lambda>' u d v) x = global_state ns x" using \<open>u \<in> ?U\<close>
+        by (simp add: \<open>map_of (fst \<Lambda>) x = Some y\<close> global_state_update_other)
+    qed
     show "update_var \<Lambda>' u d v \<in> ?U" 
       apply (simp only: initial_set.simps)
       apply (rule Set.CollectI)
       apply (intro conjI)
          apply (rule S1Upd)
       apply (rule S2Upd)
-       apply (rule Rel1Upd)
+        apply (rule Rel1Upd)
+      apply (rule GlobalConstraint)
       using update_var_binder_same Binder1 
       by metis
   qed
-
-lemma dom_map_of_2:"dom (map_of R) = set (map fst R)"
-  by (simp add: Map.dom_map_of_conv_image_fst)
 
 lemma const_rel:
   assumes Rel:"nstate_rel ((consts@globals),locals) (consts@globals2, locals2) R ns u" and
@@ -424,4 +416,75 @@ lemma injective_fun_to_list_2:
   shows "inj_on_defined R_fun"
   using assms injective_fun_to_list strictly_ordered_distinct by blast
 
+fun max_rel :: "(nat + lit) list \<Rightarrow> nat"
+  where 
+    "max_rel [] = 0"
+  | "max_rel ((Inl n) # xs) = (max n (max_rel xs))" 
+  | "max_rel ((Inr l) # xs) = (max_rel xs)"
+
+
+lemma max_rel_aux:
+  assumes "max_rel xs = w_max" and "(Inl n) \<in> set xs" 
+  shows "n \<le> w_max"
+  using assms
+  apply (induction arbitrary: n w_max rule: max_rel.induct)
+    apply simp
+   apply fastforce
+  apply simp
+  done
+
+fun max_rel_tail :: "nat \<Rightarrow> (nat + lit) list \<Rightarrow> nat"
+  where 
+    "max_rel_tail k [] = k"
+  | "max_rel_tail k ((Inl n) # xs) = (max_rel_tail (max n k) xs)" 
+  | "max_rel_tail k ((Inr l) # xs) = (max_rel_tail k xs)"
+
+lemma max_rel_tail_equiv_aux: "max_rel_tail k xs = max k (max_rel xs)"
+  by (induction arbitrary: k rule: max_rel.induct) auto
+
+lemma max_tail_equiv: "max_rel_tail 0 xs = max_rel xs"
+  by (simp add: max_rel_tail_equiv_aux)
+
+lemma rel_range_fun_to_list:
+  assumes R_fun_def:"R_fun = map_of R_list" and
+          "max_rel_tail 0 (map snd R_list) = w_max"
+  shows "\<forall>x \<in> rel_range R_fun. x \<le> w_max"
+  unfolding rel_range_def
+proof 
+  fix x
+  assume "x \<in> {y. \<exists>x. R_fun x = Some (Inl y)}"
+  from this obtain z where "R_fun z = Some (Inl x)" by auto
+  hence "map_of R_list z = Some (Inl x)" using R_fun_def by simp
+  hence "(z,Inl x) \<in> set (R_list)"
+    by (simp add: map_of_SomeD)
+  thus "x \<le> w_max" using max_tail_equiv max_rel_aux
+    by (metis assms(2) set_zip_rightD zip_map_fst_snd)
+qed
+
+
+lemma axiom_assm_aux:
+  assumes "axiom_assm A \<Gamma> consts ns1 axioms" and
+          "\<And> x y. map_of consts x = Some y \<Longrightarrow> (global_state ns1) x = (global_state ns2) x"
+        shows "axiom_assm A \<Gamma> consts ns2 axioms"
+  using assms
+  unfolding state_restriction_def
+proof -
+  have Aux:" (\<lambda>x. if map_of consts x \<noteq> None then global_state ns2 x else None) =  (\<lambda>x. if map_of consts x \<noteq> None then global_state ns1 x else None)"
+    using assms(2) by fastforce
+  show "axioms_sat A (consts, []) \<Gamma> (global_to_nstate (\<lambda>x. if map_of consts x \<noteq> None then global_state ns2 x else None)) axioms"
+    apply (subst Aux)
+    using assms(1)
+    unfolding state_restriction_def
+    apply assumption
+    done
+qed
+
+lemma helper_init_disj:
+  assumes Max1:"\<forall>x \<in> xs. x \<le> n" and "\<forall>y \<in> ys. y \<le> m" and "n < w_max" and "m < w_max"
+  shows "{w. (w :: nat) \<ge> w_max} \<inter> (xs \<union> ys) = {}"
+  using assms
+  by auto
+
+
+  
 end
